Add top-level proofs to main module

Main.v
@@ -1,19 +1,19 @@
 Require Import Grammar.
 Require Import mkParseTable_correct.
-Require Import Parser_sound.
+Require Import Parser_complete.
 
 Module Main (Import G : Grammar.T).
 
-  Module Import GeneratorProofs := GeneratorProofsFn G.
-  Module Import ParserSoundness := ParserSoundnessFn G.
+  Module Import GeneratorAndProofs := GeneratorProofsFn G.
+  Module Import ParserAndProofs    := ParserProofsFn G.
 
   Definition parseTableOf (g : grammar) : option parse_table :=
-    let nu := mkNullableSet g in
+    let nu    := mkNullableSet g in
     let nu_pf := (mkNullableSet_correct g) in
-    let fi := mkFirstMap g nu in
+    let fi    := mkFirstMap g nu in
     let fi_pf := (mkFirstMap_correct g nu nu_pf) in
-    let fo := mkFollowMap g nu fi fi_pf in
-    let es := mkEntries nu fi fo g in
+    let fo    := mkFollowMap g nu fi fi_pf in
+    let es    := mkEntries nu fi fo g in
     mkParseTable es.
 
   Theorem parseTableOf_sound : 
@@ -46,16 +46,14 @@ Module Main (Import G : Grammar.T).
     - apply mkFollowMap_correct; auto.
       apply mkNullableSet_correct; auto.
   Qed.
-  
+
   Definition parse (tbl : parse_table)
-             (sym : symbol)
-             (input : list terminal) :
+                   (sym : symbol)
+                   (input : list terminal) :
     Datatypes.sum parse_failure (tree * list terminal) :=
-    match parse_nf tbl sym input NtSet.empty
-                   (triple_lt_wf (meas tbl input NtSet.empty (F_arg sym)))
-    with
+    match parse_nf tbl sym input NtSet.empty (triple_lt_wf _) with
     | inl failure => inl failure
-    | inr (tr, existT _ input' Hle) => inr (tr, input')
+    | inr (tr, existT _ input' _) => inr (tr, input')
     end.
 
   Theorem parser_sound :
@@ -70,12 +68,59 @@ Module Main (Import G : Grammar.T).
   Proof.
     intros.
     unfold parse in *.
-    destruct (parse_nf tbl sym (word ++ rem) NtSet.empty (triple_lt_wf (meas tbl (word ++ rem) NtSet.empty (F_arg sym)))) eqn:Hp.
-    - tc.
-    - destruct p.
-      destruct s.
+    match goal with
+    | H : match ?X with | _ => _ end = _ |- _ => destruct X eqn:Hp
+    end; tc.
+    destruct p.
+    destruct s.
+    inversion H0; subst.
+    eapply parse_sound; eauto.
+  Qed.
+    
+  Theorem parse_safe :
+    forall (g   : grammar)
+           (tbl : parse_table)
+           (sym : symbol)
+           (input : list terminal)
+           (tr : tree),
+      parse_table_correct tbl g
+      -> forall x vis input',
+        ~ parse tbl sym input = inl (LeftRec x vis input').
+  Proof.
+    unfold not; intros.
+    unfold parse in H0.
+    match goal with
+    | H : match ?X with | _ => _ end = _ |- _ => destruct X eqn:Hp
+    end.
+    - destruct p; tc.
       inversion H0; subst.
-      eapply parse_sound; eauto.  
-Qed.
+      eapply leftrec_conditions with (sa := F_arg sym) in Hp; eauto.
+      destruct Hp.
+      + destruct H1.
+        ND.fsetdec.
+      + destruct H1.
+        eapply LL1_parse_table_impl_no_left_recursion; eauto.
+    - step; step; tc.
+  Qed.
 
+  Theorem parse_complete :
+    forall g tbl sym word tr rem,
+      parse_table_correct tbl g
+      -> (@sym_derives_prefix g) sym word tr rem
+      -> parse tbl sym (word ++ rem) = inr (tr, rem).
+  Proof.
+    intros.
+    eapply parse_nf_complete_or_leftrec in H0; eauto.
+    destruct H0.
+    - exfalso.
+      destruct H0 as [x [vis [input' Hp]]].
+      eapply parse_safe; eauto.
+      unfold parse.
+      rewrite Hp; eauto.
+    - destruct H0 as [Hle Hp].
+      unfold parse.
+      rewrite Hp; auto.
+  Qed.
+  
 End Main.
+
